theories/layout.v
@@ -139,6 +139,11 @@ Definition float_type_type (νf : float_type) : type :=
   let ι := float_type_rep νf in
   NumT (VALTYPE (PrimR ι) ImCopy ImDrop) (FloatT νf).
 
+Definition type_i32 : type := int_type_type I32T.
+Definition type_i64 : type := int_type_type I64T.
+Definition type_f32 : type := float_type_type F32T.
+Definition type_f64 : type := float_type_type F64T.
+
 (* Fact: If |- NumT ν : κ, then Some [num_type_rep ν] = type_rep (NumT ν). *)
 Definition num_type_rep (ν : num_type) : primitive_rep :=
   match ν with
